change definitions, prove most of cur_request<->timeout recv case

systems/chord-props/QueryInvariant.v
@@ -170,6 +170,14 @@ Theorem at_most_one_request_timeout_invariant :
 Proof.
 Admitted.
 
+(* TODO(ryan) move to Chord.v *)
+Definition query_response_dec :
+  forall q p,
+    {query_response q p} + {~ query_response q p}.
+Proof.
+  destruct p, q; solve [auto | right; intro H; inv H].
+Defined.
+
 Lemma recv_msg_not_right_response_preserves_cur_request :
   forall src dst st p st' ms nts cts,
     recv_handler src dst st p = (st', ms, nts, cts) ->
@@ -186,65 +194,65 @@ Proof.
     intuition.
 Qed.
 
-Hint Resolve live_node_characterization.
-
-Inductive cur_request_timeouts_related (gst : global_state) (h : addr) : Prop :=
-| QSTNoRequest :
-    forall st,
-      sigma gst h = Some st ->
-      (forall dst req, ~ In (Request dst req) (timeouts gst h)) ->
-      cur_request st = None ->
-      cur_request_timeouts_related gst h
-| QSTRequest :
-    forall st dstp q req,
-      sigma gst h = Some st ->
-      query_request q req ->
-      In (Request (addr_of dstp) req) (timeouts gst h) ->
+Lemma recv_msg_not_right_response_never_removes_request_timeout :
+  forall src dst st p st' ms nts cts,
+    recv_handler src dst st p = (st', ms, nts, cts) ->
+    forall dstp q req,
       cur_request st = Some (dstp, q, req) ->
-      cur_request_timeouts_related gst h.
-Hint Constructors cur_request_timeouts_related.
-
-Lemma cur_request_timeouts_related_equiv_st :
-  forall gst gst' h,
-    sigma gst h = sigma gst' h ->
-    timeouts gst h = timeouts gst' h ->
-    cur_request_timeouts_related gst h ->
-    cur_request_timeouts_related gst' h.
+      ~ query_response q p ->
+      In (Request (addr_of dstp) req) nts \/
+      ~ In (Request (addr_of dstp) req) cts.
 Proof.
   intros.
-  inv_prop cur_request_timeouts_related;
-    repeat find_rewrite; eauto.
+  repeat (handler_def || handler_simpl);
+    repeat (find_rewrite || find_injection);
+    solve [tauto | find_false; intuition].
 Qed.
 
-Definition live_node_cur_request_timeouts_related (gst : global_state) : Prop :=
-  forall h,
+Inductive cur_request_timeouts_ok (cr : option (pointer * query * payload)) (ts : list timeout) : Prop :=
+| QSTNoRequest :
+    (forall dst req, ~ In (Request dst req) ts) ->
+    cr = None ->
+    cur_request_timeouts_ok cr ts
+| QSTRequest :
+    forall dstp q req,
+      query_request q req ->
+      In (Request (addr_of dstp) req) ts ->
+      cr = Some (dstp, q, req) ->
+      cur_request_timeouts_ok cr ts.
+Hint Constructors cur_request_timeouts_ok.
+
+Definition all_nodes_cur_request_timeouts_related (gst : global_state) : Prop :=
+  forall h st,
     In h (nodes gst) ->
     ~ In h (failed_nodes gst) ->
-    cur_request_timeouts_related gst h.
-Hint Unfold live_node_cur_request_timeouts_related.
+    sigma gst h = Some st ->
+    cur_request_timeouts_ok (cur_request st) (timeouts gst h).
+Hint Unfold all_nodes_cur_request_timeouts_related.
 
 Lemma cur_request_timeouts_related_recv_invariant :
-  chord_recv_handler_invariant live_node_cur_request_timeouts_related.
+  chord_recv_handler_invariant all_nodes_cur_request_timeouts_related.
 Proof.
   autounfold; intros.
   destruct (addr_eq_dec h0 h).
   - subst; rewrite_update.
-    assert (cur_request_timeouts_related gst h)
+    assert (cur_request_timeouts_ok (cur_request st) (timeouts gst h))
       by (repeat find_rewrite; auto).
     find_copy_eapply_lem_hyp recv_handler_possible_nts.
     find_copy_eapply_lem_hyp recv_handler_possible_cts.
-    inv_prop cur_request_timeouts_related.
+    assert (st0 = st')
+      by (repeat find_rewrite; rewrite_update; congruence);
+      subst.
+    inv_prop cur_request_timeouts_ok.
     + destruct nts.
       * destruct (cur_request st') as [[[? ?] ?]|] eqn:?.
-        -- (* need lemma like handle_query_res_info_from_changed_set_cur_request
-              but for recv_handler *)
-          admit.
+        -- repeat (handler_def || handler_simpl).
         -- econstructor; eauto;
              repeat find_rewrite; rewrite_update; simpl; auto.
            autounfold; intros.
            find_apply_lem_hyp in_remove_all_was_in.
            cut (~ In (Request dst req) (timeouts gst h)); [intuition|].
-           inv_prop cur_request_timeouts_related; eauto.
+           inv_prop cur_request_timeouts_ok; eauto.
       * repeat (handler_def || handler_simpl ||
                 match goal with
                 | H : context[recv_handler] |- _ =>
@@ -259,11 +267,14 @@ Proof.
         autounfold; intros; simpl in *; break_or_hyp; try congruence.
         cut (In (Request dst req) (timeouts gst h)); [eauto|].
         eapply in_remove; eauto.
-    + admit.
-  - assert (cur_request_timeouts_related gst h0) by (repeat find_rewrite; auto).
-    find_eapply_lem_hyp cur_request_timeouts_related_equiv_st; eauto;
-      repeat find_rewrite; rewrite_update; reflexivity.
-Admitted.
+    + destruct (query_response_dec q p).
+      * admit.
+      * find_copy_eapply_lem_hyp recv_msg_not_right_response_preserves_cur_request; eauto.
+        find_eapply_lem_hyp recv_msg_not_right_response_never_removes_request_timeout; eauto.
+        repeat find_rewrite; rewrite_update.
+        intuition eauto using in_remove_all_preserve with datatypes.
+  - repeat find_rewrite; rewrite_update; eauto.
+Qed.
 
 Lemma open_request_with_response_on_wire_closed_or_preserved :
   forall gst l gst' src dst req res,
